Allow giving only one binder name and retriviing it in the phoas representation

pcuic/theories/PCUICPHOAS.v
@@ -1,16 +1,21 @@
 From Coq Require Import String List ZArith.
-From MetaCoq.Template Require config utils All.
-From MetaCoq.Template Require Import BasicAst TemplateMonad monad_utils.
+From MetaCoq.Template Require config utils.
+From MetaCoq.Template Require Import All Loader.
+From MetaCoq.Template Require Import bytestring BasicAst TemplateMonad monad_utils.
 From MetaCoq.PCUIC Require Import TemplateToPCUIC.
 Import MCMonadNotation.
-Local Open Scope string_scope.
 Import ListNotations.
 
+Open Scope bs.
 (* From MetaCoq.PCUIC Require Import PCUICAst PCUICReduction PCUICCumulativity PCUICTyping PCUICSafeLemmata. *)
+
+Notation " f $ x " := (f x) (only parsing, at level 10, x at level 20).
 
 From MetaCoq.Template Require Import Universes.
 Declare Custom Entry term.
 Module LevelsToIndices.
+
+
 Import Ast.
 
 (* Conversion from de Bruijn levels to indices *)
@@ -27,7 +32,9 @@ Fixpoint toDB k (t : term) : term :=
   | tConst c u => Ast.tConst c u
   | tInd c u => Ast.tInd c u
   | tConstruct c k u => Ast.tConstruct c k u
-  | _ => Ast.tInt (Int63.of_Z 0%Z)
+  | tLetIn na b t t' => Ast.tLetIn na (toDB k b) (toDB k t) (toDB (S k) t')
+  | _ => Ast.tVar "not supported"%bs
+  (* | _ => Ast.tInt (Int63.of_Z 0%Z) *)
   end.
 End LevelsToIndices.
 
@@ -38,9 +45,9 @@ Inductive term {var : Type} | : Type :=
 | tEvar (ev : nat) (args : list term)
 | tSort (s : Universe.t)
 | tCast (t : term) (kind : cast_kind) (v : term)
-| tProd (na : aname) (ty : term) (body : var -> term)
-| tLambda (na : aname) (ty : term) (body : var -> term)
-| tLetIn (na : aname) (def : term) (def_ty : term) (body : var -> term)
+| tProd (r : relevance) (ty : term) (body : var -> term)
+| tLambda (r : relevance) (ty : term) (body : var -> term)
+| tLetIn (r : relevance) (def : term) (def_ty : term) (body : var -> term)
 | tApp (f : term) (args : list term)
 | tConst (c : kername) (u : Instance.t)
 | tInd (ind : inductive) (u : Instance.t)
@@ -49,10 +56,67 @@ Inductive term {var : Type} | : Type :=
         (discr:term) (branches : list (nat * term))
 | tProj (proj : projection) (t : term)
 | tFix (mfix : mfixpoint term) (idx : nat)
-| tCoFix (mfix : mfixpoint term) (idx : nat)
-| tInt (i : Int63.int)
-| tFloat (f : PrimFloat.float).
+| tCoFix (mfix : mfixpoint term) (idx : nat).
+(* | tInt (i : Int63.int) *)
+(* | tFloat (f : PrimFloat.float). *)
 Arguments term : clear implicits.
+
+Definition get_binder_name {var} (fn : var -> term var) : TemplateMonad name :=
+  fnast <- tmQuote fn ;;
+  match fnast with
+  | Ast.tLambda na _ _ => ret $ binder_name na
+  | _ => tmFail "not a binder"
+  end.
+
+(* To de Bruijn indices *)
+Fixpoint toDB k (t : term nat) : TemplateMonad Ast.term :=
+  match t with 
+  | tRel n => ret (Ast.tRel (k - S n))
+  | tVar id => ret (Ast.tVar id)
+  | tEvar ev args =>
+    args' <- monad_map (toDB k) args ;;
+    ret (Ast.tEvar ev args')
+  | tSort s => ret (Ast.tSort s)
+  | tCast t ck u => 
+    t' <- (toDB k t) ;;
+    u' <- toDB k u ;;
+    ret (Ast.tCast t' ck u')
+  | tProd rel ty body =>
+    ty' <- toDB k ty ;;
+    na <- get_binder_name body ;;
+    body' <- toDB (S k) (body k) ;;
+    ret (Ast.tProd {| binder_relevance := rel; binder_name := na |} ty' body')
+  | tLambda rel ty body =>
+    ty' <- toDB k ty ;;
+    na <- get_binder_name body ;;
+    body' <- toDB (S k) (body k) ;;
+    ret (Ast.tLambda {| binder_relevance := rel; binder_name := na |} ty' body')
+  | tLetIn rel ty b body => 
+    ty' <- toDB k ty ;;
+    b' <- toDB k b ;;
+    na <- get_binder_name body ;;
+    body' <- toDB (S k) (body k) ;;
+    ret (Ast.tLetIn {| binder_relevance := rel; binder_name := na |} ty' b' body')
+  | tApp f args =>
+    f' <- toDB k f ;;
+    args' <- monad_map (toDB k) args ;;
+    ret (Ast.tApp f' args')
+  | tConst c u => ret $ Ast.tConst c u
+  | tInd c u => ret $ Ast.tInd c u
+  | tConstruct c k u => ret $ Ast.tConstruct c k u
+  | tCase i t d brs => tmFail "not supported"%bs
+    (* ret $ Ast.tCase i (toDB k t) (toDB k d) (List.map (fun '(x, y) => (x, toDB k y)) brs) *)
+  | tProj p t => t' <- toDB k t ;; ret $ Ast.tProj p t'
+  | tFix mfix idx => tmFail "not supported"%bs
+    (* let mfix' := List.map (map_def (toDB k) (toDB (k + length mfix))) mfix in *)
+    (* Ast.tFix mfix' idx *)
+  | tCoFix mfix idx => tmFail "not supported"%bs
+    (* let mfix' := List.map (map_def (toDB k) (toDB (k + length mfix))) mfix in *)
+    (* Ast.tCoFix mfix' idx *)
+  (* | tInt i => Ast.tInt i *)
+  (* | tFloat f => Ast.tFloat f *)
+  end.
+(* 
 
 (* To de Bruijn indices *)
 Fixpoint toDB k (t : term nat) : Ast.term :=
@@ -62,7 +126,7 @@ Fixpoint toDB k (t : term nat) : Ast.term :=
   | tEvar ev args => Ast.tEvar ev (List.map (toDB k) args)
   | tSort s => Ast.tSort s
   | tCast t ck u => Ast.tCast (toDB k t) ck (toDB k u)
-  | tProd na ty body => Ast.tProd na (toDB k ty) (toDB (S k) (body k))
+  | tProd na ty body => Ast.tProd {| binder_relevance := na |} (toDB k ty) (toDB (S k) (body k))
   | tLambda na ty body => Ast.tLambda na (toDB k ty) (toDB (S k) (body k))
   | tLetIn na ty b body => Ast.tLetIn na (toDB k ty) (toDB k b) (toDB (S k) (body k))
   | tApp f args => Ast.tApp (toDB k f) (List.map (toDB k) args)
@@ -78,11 +142,11 @@ Fixpoint toDB k (t : term nat) : Ast.term :=
   | tCoFix mfix idx => 
     let mfix' := List.map (map_def (toDB k) (toDB (k + length mfix))) mfix in
     Ast.tCoFix mfix' idx
-  | tInt i => Ast.tInt i
-  | tFloat f => Ast.tFloat f
-  end.
+  (* | tInt i => Ast.tInt i *)
+  (* | tFloat f => Ast.tFloat f *)
+  end. *)
 
-  Definition tImpl {var} (A B : term var) := tProd bAnon A (fun _ => B).
+  Definition tImpl {var} (A B : term var) := tProd Relevant A (fun _ => B).
 End PHOAS.
 Definition term := forall var, PHOAS.term var.
 
@@ -98,10 +162,9 @@ Notation "t1 t2" := (PHOAS.tApp t1 [t2]) (in custom term at level 4, left associ
 Notation "'Type' u" := (PHOAS.tSort u) (u constr, in custom term at level 0).
 Notation "'Type0'" := (PHOAS.tSort Universe.type0) (in custom term at level 0).
 Notation "'Type1'" := (PHOAS.tSort Universe.type1) (in custom term at level 0).
-Notation "'Π' x @ ( na , A ) , B" := (PHOAS.tProd (bNamed na) A (fun x => B))
+Notation "'Π' x : A , B" := (PHOAS.tProd Relevant A (fun x => B))
                          (in custom term at level 4, right associativity,
                              x binder,
-                             na constr,
                              A custom term at level 4,
                              B custom term at level 4).
 Notation "A → B" := (PHOAS.tImpl A B)
@@ -109,27 +172,37 @@ Notation "A → B" := (PHOAS.tImpl A B)
     A custom term,
     B custom term at level 4).
     
-Notation "'λ' x @ ( na , A ) , B" := (PHOAS.tLambda (bNamed na) A (fun x : _ => B)) 
+Notation "'λ' x :: A , B" := (PHOAS.tLambda Relevant A (fun x : _ => B)) 
   (in custom term at level 4, right associativity,
   x binder,
-  na constr,
   A custom term at level 4,
   B custom term at level 4).
 
 Notation "' x" := (PHOAS.tRel x) (in custom term at level 0, x constr at level 2, format "' x").
 Notation "{ x }" := x (x constr, in custom term).
 
-Definition of_phoas (t : myterm) : PCUICAst.term := 
-  TemplateToPCUIC.trans (PHOAS.toDB 0 t).
+Global Hint Mode Monad ! : typeclass_instances.
 
-Coercion of_phoas : myterm >-> PCUICAst.term.
+Import PCUICProgram.
+
+Definition of_phoas (t : myterm) : TemplateMonad PCUICAst.term := 
+  let envmap := build_global_env_map PCUICAst.PCUICEnvironment.empty_global_env in
+  t' <- PHOAS.toDB 0 t ;; ret $ TemplateToPCUIC.trans envmap t'.
+
+(* Coercion of_phoas : myterm >-> PCUICAst.term. *)
 
 Coercion nat_rel : nat >-> myterm.
 
-(* Definition tnat {var} : PHOAS.term var  := PHOAS.tInd
+Definition tnat {var} : PHOAS.term var  := PHOAS.tInd
   {|
   	inductive_mind := (MPfile ["Datatypes"; "Init"; "Coq"], "nat");
     inductive_ind := 0
-  |} []. *)
+  |} [].
 
-(* Type [! λ x @ ("x", { tnat }), λ x' @ ("x", { tnat }), λ y @ ("y", Type0), 'y 'x]. *)
+Notation "'nat'" := tnat (in custom term).
+
+Example ex1 := [! λ x :: nat, λ x' :: {tnat}, λ y :: Type0, 'y 'x].
+
+MetaCoq Run (of_phoas ex1 >>= tmEval all >>= tmDefinition "qex1").
+
+Type [! λ x :: nat, λ x' :: nat, λ y :: Type0, 'y 'x].
